Attempt to add Thunk into data_to_word invariants

compiler/backend/proofs/data_to_word_memoryProofScript.sml
@@ -131,7 +131,12 @@ QED
 (* -- *)
 
 Datatype:
-  tag = BlockTag num | RefTag | BytesTag bool num | NumTag bool | Word64Tag
+  tag = BlockTag num         (* immutable Block                         *)
+      | RefTag               (* mutable arrays / references             *)
+      | BytesTag bool num    (* mutable byte arrays / immutable strings *)
+      | ThunkTag thunk_mode  (* mutable thunks                          *)
+      | NumTag bool          (* immutable bignum on the heap            *)
+      | Word64Tag            (* immutable word64 on the heap            *)
 End
 
 Definition BlockRep_def:
@@ -234,34 +239,43 @@ Definition ref_edge_def:
   ref_edge refs (x:num) (y:num) =
     case lookup x refs of
     | SOME (ValueArray ys) => MEM y (get_refs (Block 0 ARB ys))
+    | SOME (Thunk _ v) => MEM y (get_refs (Block 0 ARB [v]))
     | _ => F
 End
 
 Definition reachable_refs_def:
   reachable_refs roots refs t =
-    ?x r. MEM x roots /\ MEM r (get_refs x) /\ RTC (ref_edge refs) r t
+    ∃x r. MEM x roots ∧ MEM r (get_refs x) ∧ RTC (ref_edge refs) r t
 End
 
 Definition RefBlock_def:
   RefBlock xs = DataElement xs (LENGTH xs) (RefTag,[])
 End
 
+Definition ThunkBlock_def:
+  ThunkBlock ev x = DataElement [x] 1 (ThunkTag ev,[])
+End
+
 Definition bc_ref_inv_def:
   bc_ref_inv conf n refs (f,tf,heap,be) =
     case (FLOOKUP f n, lookup n refs) of
     | (SOME x, SOME (ValueArray ys)) =>
-        (?zs. (heap_lookup x heap = SOME (RefBlock zs)) /\
-              EVERY2 (\z y. v_inv conf y (z,f,tf,heap)) zs ys)
+        (∃zs. heap_lookup x heap = SOME (RefBlock zs) ∧
+              EVERY2 (λz y. v_inv conf y (z,f,tf,heap)) zs ys)
     | (SOME x, SOME (ByteArray flag bs)) =>
         let ws = LENGTH bs DIV (dimindex (:α) DIV 8) + 1 in
           (heap_lookup x heap = SOME (Bytes be flag bs (REPLICATE ws (0w:'a word))))
+    | (SOME x, SOME (Thunk ev v)) =>
+        (∃(z:α word_loc heap_address).
+           heap_lookup x heap = SOME (ThunkBlock ev z) ∧
+           v_inv conf v (z,f,tf,heap))
     | _ => F
 End
 
 (* TODO: MOVE *)
 Definition v_all_ts_def:
-  v_all_ts (Block ts _ xs) = ts :: FLAT (MAP v_all_ts xs)
-∧ v_all_ts _ = []
+  v_all_ts (Block ts _ xs) = ts :: FLAT (MAP v_all_ts xs) ∧
+  v_all_ts _ = []
 Termination
   WF_REL_TAC `measure (v_size)` \\ rpt strip_tac \\ Induct_on `xs`
   \\ srw_tac [] [v_size_def] \\ res_tac \\ DECIDE_TAC
@@ -303,8 +317,12 @@ Definition unused_space_inv_def:
     data_up_to ptr heap
 End
 
+Definition isMutTag_def:
+  isMutTag t ⇔ t = RefTag ∨ ∃ev. t = ThunkTag ev
+End
+
 Definition isRef_def:
-  isRef (DataElement ys l (tag,qs)) = (tag = RefTag) /\
+  isRef (DataElement ys l (tag,qs)) = isMutTag tag ∧
   isRef _ = F
 End
 
@@ -587,8 +605,13 @@ Proof
   \\ Cases_on `lookup n refs` \\ full_simp_tac (srw_ss()) []
   \\ full_simp_tac (srw_ss()) [FLOOKUP_DEF,f_o_f_DEF]
   \\ Cases_on `x'` \\ full_simp_tac (srw_ss()) []
-  \\ TRY (fs[Bytes_def,LET_THM] >> res_tac >> simp[ADDR_MAP_def]
-          \\ rw [] \\ qexists_tac `ws` \\ fs [] >> NO_TAC)
+  >~ [‘lookup n refs = SOME (ByteArray b l)’] >-
+   (fs[Bytes_def,LET_THM] \\ res_tac \\ simp[ADDR_MAP_def]
+    \\ rw [] \\ qexists_tac `ws` \\ fs [])
+  >~ [‘lookup n refs = SOME (Thunk ev v)’] >-
+   (fs [ThunkBlock_def]
+    \\ res_tac \\ fs []
+    \\ cheat)
   \\ res_tac \\ full_simp_tac (srw_ss()) [LENGTH_ADDR_MAP,EVERY2_ADDR_MAP]
   \\ rpt strip_tac \\ qpat_x_assum `EVERY2 qqq zs l` MP_TAC
   \\ match_mp_tac EVERY2_IMP_EVERY2 \\ simp_tac std_ss [] \\ rpt strip_tac
@@ -602,6 +625,7 @@ Triviality RTC_lemma:
           gc_shared$gc_related g heap heap2 /\
           f ' r IN FDOM g ==> f ' n IN FDOM g
 Proof
+  cheat (*
   ho_match_mp_tac RTC_INDUCT \\ full_simp_tac std_ss [] \\ rpt strip_tac
   \\ full_simp_tac std_ss []
   \\ qpat_x_assum `bb ==> bbb` match_mp_tac \\ full_simp_tac std_ss []
@@ -627,7 +651,7 @@ Proof
   \\ res_tac \\ CCONTR_TAC \\ full_simp_tac std_ss []
   \\ srw_tac [] [] \\ POP_ASSUM MP_TAC \\ simp_tac std_ss []
   \\ imp_res_tac MEM_EVERY2_IMP \\ fs []
-  \\ fs [] \\ metis_tac []
+  \\ fs [] \\ metis_tac [] *)
 QED
 
 Triviality reachable_refs_lemma:
@@ -692,8 +716,8 @@ Definition all_reachable_from_roots_def:
        p IN reachable_addresses roots heap
 End
 
-val IN_reachable_addresses =
-  ``x ∈ reachable_addresses roots heap``
+Triviality IN_reachable_addresses =
+  “x ∈ reachable_addresses roots heap”
   |> SIMP_CONV std_ss [Once IN_DEF,reachable_addresses_def]
 
 Theorem reachable_addresses_related:
@@ -811,13 +835,12 @@ QED
 
 Definition make_gc_conf_def:
   make_gc_conf limit =
-    <| limit := limit; isRef := \x. FST x = RefTag |>
-        : (tag # 'a) gen_gc$gen_gc_conf
+    <| limit := limit; isRef := isMutTag o FST |> : (tag # 'a) gen_gc$gen_gc_conf
 End
 
 Triviality gc_move_data_refs_split:
-  (gen_gc$gc_move cc s x = (x1,s1)) /\ (!t r. (cc.isRef (t,r) <=> t = RefTag))
-   /\ EVERY isDataElement s.h2 /\(EVERY (λx. ¬isRef x)) s.h2 /\ EVERY isRef s.r4 ==>
+  (gen_gc$gc_move cc s x = (x1,s1)) /\ (∀t r. cc.isRef (t,r) <=> isMutTag t) /\
+   EVERY isDataElement s.h2 /\ EVERY (λx. ¬isRef x) s.h2 /\ EVERY isRef s.r4 ==>
    EVERY isDataElement s1.h2 /\
    (EVERY (λx. ¬isRef x)) s1.h2 /\ EVERY isRef s1.r4
 Proof
@@ -831,7 +854,7 @@ QED
 
 Triviality gc_move_list_data_refs_split:
   !x x1 s s1.
-  (gen_gc$gc_move_list cc s x = (x1,s1)) /\ (!t r. (cc.isRef (t,r) <=> t = RefTag))
+  (gen_gc$gc_move_list cc s x = (x1,s1)) /\ (!t r. (cc.isRef (t,r) <=> isMutTag t))
    /\ EVERY isDataElement s.h2 /\(EVERY (λx. ¬isRef x)) s.h2 /\ EVERY isRef s.r4 ==>
    EVERY isDataElement s1.h2 /\(EVERY (λx. ¬isRef x)) s1.h2 /\ EVERY isRef s1.r4
 Proof
@@ -842,7 +865,7 @@ QED
 
 Triviality gc_move_refs_data_refs_split:
   !cc s s1.
-  (gen_gc$gc_move_refs cc s = s1) /\ (!t r. (cc.isRef (t,r) <=> t = RefTag))
+  (gen_gc$gc_move_refs cc s = s1) /\ (!t r. (cc.isRef (t,r) <=> isMutTag t))
    /\ EVERY isDataElement (s.h1++s.h2) /\ (EVERY (λx. ¬isRef x)) (s.h1++s.h2) /\
    EVERY isRef (s.r1 ++ s.r2 ++ s.r3 ++ s.r4) ==>
    EVERY isDataElement (s1.h1++s1.h2) /\
@@ -864,7 +887,7 @@ QED
 
 Triviality gc_move_data_data_refs_split:
   !cc s s1.
-  (gen_gc$gc_move_data cc s = s1) /\ (!t r. (cc.isRef (t,r) <=> t = RefTag))
+  (gen_gc$gc_move_data cc s = s1) /\ (!t r. (cc.isRef (t,r) <=> isMutTag t))
    /\ (EVERY (λx. ¬isRef x)) (s.h1++s.h2) /\
    EVERY isDataElement (s.h1++s.h2) /\
    EVERY isRef (s.r1 ++ s.r2 ++ s.r3 ++ s.r4) ==>
@@ -887,7 +910,7 @@ QED
 Triviality gc_move_loop_data_refs_split:
   !clock cc s s1.
   (gen_gc$gc_move_loop cc s clock = s1) /\
-  (!t r. (cc.isRef (t,r) <=> t = RefTag)) /\
+  (!t r. (cc.isRef (t,r) <=> isMutTag t)) /\
   EVERY isDataElement (s.h1++s.h2) /\
   (EVERY (λx. ¬isRef x)) (s.h1++s.h2) /\
   EVERY isRef (s.r1 ++ s.r2 ++ s.r3 ++ s.r4) ==>
@@ -913,7 +936,7 @@ QED
 Triviality gen_gc_data_refs_split:
   !cc roots heap.
   (gen_gc cc (roots,heap) = (roots1,s)) /\
-  (!t r. (cc.isRef (t,r) <=> t = RefTag)) ==>
+  (!t r. (cc.isRef (t,r) <=> isMutTag t)) ==>
   (EVERY (λx. ¬isRef x)) (s.h1 ++ s.h2) /\
   EVERY isDataElement (s.h1 ++ s.h2) /\
   EVERY isRef (s.r1 ++ s.r2 ++ s.r3 ++ s.r4)
@@ -1171,6 +1194,7 @@ Proof
      (fs [EVERY_MEM] \\ CCONTR_TAC \\ fs []
       \\ Cases_on `x` \\ fs [isRef_def]
       \\ Cases_on `b` \\ fs [isRef_def] \\ rveq
+      \\ gvs [isMutTag_def]
       \\ res_tac \\ fs [] \\ res_tac \\ fs [])
     \\ fs [EVERY_MEM] \\ CCONTR_TAC \\ fs []
     \\ qpat_x_assum `MEM e _` (assume_tac o REWRITE_RULE [MEM_SPLIT])
@@ -1180,10 +1204,10 @@ Proof
     \\ rveq \\ fs[]
     \\ `isRef x` by metis_tac []
     \\ Cases_on `x` \\ fs [isRef_def]
-    \\ Cases_on `b` \\ fs [isRef_def]
+    \\ Cases_on `b` \\ fs [isRef_def,isMutTag_def]
     \\ Cases_on `e` \\ rveq
     \\ fs [gen_gc_partialTheory.similar_data_def,isRef_def]
-    \\ rveq \\ fs[isRef_def])
+    \\ rveq \\ fs[isRef_def,isMutTag_def])
   \\ fs [roots_ok_def]
   \\ rpt strip_tac
   \\ imp_res_tac MEM_ADDR_MAP
@@ -1752,10 +1776,11 @@ Theorem isDataElement_lemmas[simp]:
     isDataElement (Word64Rep (:'a) w) /\
     isDataElement (RefBlock ws) /\
     isDataElement (Bytes y1 y2 y3 y4) /\
+    isDataElement (ThunkBlock ev v) /\
     isDataElement (Bignum i)
 Proof
   rw [BlockRep_def,isDataElement_def,Bignum_def,i2mw_def,
-    Word64Rep_def,RefBlock_def,Bytes_def]
+      Word64Rep_def,RefBlock_def,Bytes_def,ThunkBlock_def]
 QED
 
 (* --- Allocating multiple cons-elements in one go --- *)
@@ -1834,7 +1859,7 @@ Theorem list_to_BlockReps_Ref:
      xs <> [] ==> EVERY (\v. ~isRef v) (list_to_BlockReps conf x len xs)
 Proof
   Induct \\ rw [list_to_BlockReps_def, BlockRep_def]
-  \\ TRY CASE_TAC \\ fs [isRef_def]
+  \\ TRY CASE_TAC \\ fs [isRef_def,isMutTag_def]
 QED
 
 Theorem list_to_BlockReps_NULL:
@@ -1897,8 +1922,7 @@ Theorem list_to_BlockReps_Pointer =
 Theorem list_to_v_get_refs:
    !xs t r ts.
      MEM r (get_refs (list_to_v ts t xs)) ==>
-
-       ?x. (MEM x xs \/ x = t) /\ MEM r (get_refs x)
+       ∃x. (MEM x xs \/ x = t) /\ MEM r (get_refs x)
 Proof
   Induct \\ rw [dataSemTheory.list_to_v_def]
   \\ fs [get_refs_def] \\ metis_tac []
@@ -2153,8 +2177,10 @@ Definition v_all_vs_def:
 End
 
 Definition all_vs_def:
-  all_vs refs stack = { v | ∃(n:num) l. lookup n refs = SOME (ValueArray l) ∧ MEM v (v_all_vs l)} ∪
-                      { v | MEM v (v_all_vs stack)}
+  all_vs refs stack =
+    { v | ∃(n:num) l. lookup n refs = SOME (ValueArray l) ∧ MEM v (v_all_vs l)} ∪
+    { v | ∃n ev x. lookup n refs = SOME (Thunk ev x) ∧ MEM v (v_all_vs [x])} ∪
+    { v | MEM v (v_all_vs stack)}
 End
 
 Theorem v_all_vs_MEM:
@@ -2180,6 +2206,7 @@ Theorem v_in_all_vs:
     x ∈ all_vs refs stack ∧ MEM y (v_all_vs [x])
     ⇒ y ∈ all_vs refs stack
 Proof
+  cheat (*
   rw [all_vs_def]
   >- (disj1_tac
      \\ cases_on `x` \\ fs [v_all_vs_def]
@@ -2190,7 +2217,7 @@ Proof
   >- (disj2_tac
      \\ cases_on `x` \\ fs [v_all_vs_def]
      \\ drule_then ASSUME_TAC v_all_vs_MEM
-     \\ fs [])
+     \\ fs []) *)
 QED
 
 Theorem v_all_vs_MEM2:
@@ -2258,6 +2285,7 @@ Theorem MEM_in_all_ts:
     x ∈ all_vs refs stack ∧ MEM ts (v_all_ts x)
     ⇒ ts ∈ all_ts refs stack
 Proof
+  cheat (*
   Cases \\  rw [all_vs_def,all_ts_def,v_all_ts_def]
   >- (drule_then ASSUME_TAC v_all_vs_MEM2 \\ fs []
      \\ drule_then ASSUME_TAC v_all_vs_ts \\ fs []
@@ -2280,7 +2308,7 @@ Proof
      \\ `MEM a (v_all_vs [Block n0 n l])` by rw [v_all_vs_def,MEM_v_all_vs]
      \\ `MEM a (v_all_vs [x])`            by metis_tac [v_all_vs_trans]
      \\ `MEM ts (v_all_ts x)`             by metis_tac [v_all_vs_ts_MEM]
-     \\ metis_tac [])
+     \\ metis_tac []) *)
 QED
 
 Theorem MEM_in_all_vs:
@@ -2380,15 +2408,17 @@ Proof
      \\ rveq \\ fs [])
 QED
 
+Triviality v_inv_ind_alt =
+  v_inv_ind |> Q.SPEC `λv (x,f,tf,heap). P v x f tf heap`
+            |> SIMP_RULE std_ss []
+            |> Q.GEN `P`;
+
 Theorem v_inv_tf_restrict:
   ∀v y f tf heap conf P.
      v_inv conf v (y,f,tf,heap) ∧ (∀x. MEM x (v_all_ts v) ⇒ x ∈ P)
      ⇒ v_inv conf v (y,f, DRESTRICT tf P,heap)
 Proof
-  let val ind = theorem "v_inv_ind" |> Q.SPEC `λv (x,f,tf,heap). P v x f tf heap`
-                                    |> SIMP_RULE std_ss []
-                                    |> Q.GEN `P`
-  in ho_match_mp_tac ind end
+  ho_match_mp_tac v_inv_ind_alt
   \\ rw [v_inv_def]
   \\ every_case_tac \\ fs []
   \\ qexists_tac `xs` \\ rw []
@@ -2514,9 +2544,13 @@ Proof
   \\ rpt strip_tac \\ full_simp_tac std_ss [RefBlock_def]
   \\ Cases_on `FLOOKUP f n` \\ full_simp_tac (srw_ss()) []
   \\ Cases_on `lookup n refs` \\ full_simp_tac (srw_ss()) []
-  \\ Cases_on `x'` \\ full_simp_tac (srw_ss()) []
-  THEN1 (
-    imp_res_tac heap_store_rel_lemma \\ full_simp_tac (srw_ss()) []
+  \\ rename [‘lookup n refs = SOME x_ref’]
+  \\ Cases_on ‘x_ref’ \\ full_simp_tac (srw_ss()) []
+  >~ [‘lookup n refs = SOME (ByteArray b1 l1)’] >-
+   (fs[Bytes_def,LET_THM] >> imp_res_tac heap_store_rel_lemma
+    \\ metis_tac [])
+  >~ [‘lookup n refs = SOME (ValueArray array_vals)’] >-
+   (imp_res_tac heap_store_rel_lemma \\ full_simp_tac (srw_ss()) []
     \\ qpat_x_assum `EVERY2 PP zs l` MP_TAC
     \\ match_mp_tac EVERY2_IMP_EVERY2 \\ full_simp_tac (srw_ss()) []
     \\ rpt strip_tac \\ res_tac
@@ -2524,8 +2558,13 @@ Proof
     \\ match_mp_tac (GEN_ALL v_inv_SUBMAP)
     \\ goal_assum (first_x_assum o mp_then Any mp_tac)
     \\ fs [])
-  \\ fs[Bytes_def,LET_THM] >> imp_res_tac heap_store_rel_lemma
-  \\ metis_tac []
+  >~ [‘lookup n refs = SOME (Thunk ev thunk_v)’] >-
+   (fs [ThunkBlock_def]
+    \\ imp_res_tac heap_store_rel_lemma \\ full_simp_tac (srw_ss()) []
+    \\ match_mp_tac v_inv_tf_update_thm \\ asm_rewrite_tac []
+    \\ match_mp_tac (GEN_ALL v_inv_SUBMAP)
+    \\ goal_assum (first_x_assum o mp_then Any mp_tac)
+    \\ fs [])
 QED
 
 Theorem cons_thm_EMPTY:
@@ -2562,6 +2601,7 @@ Theorem word64_alt_thm:
        (Pointer a (Word 0w)::roots,heap2,
         be,a + len + 1,sp - len - 1,sp1,gens) limit ts
 Proof
+  cheat (*
   rw[abs_ml_inv_def]
   \\ qpat_abbrev_tac`wr = DataElement _ _ _`
   \\ `el_length wr = len + 1`
@@ -2666,7 +2706,7 @@ Proof
        \\ map_every qexists_tac [`n`,`l`] \\ rw []
        \\ ho_match_mp_tac MEM_v_all_vs
        \\ drule MEM_ZIP2 \\ rw []
-       \\ rw [EL_MEM])
+       \\ rw [EL_MEM]) *)
 QED
 
 (* bignum *)
@@ -2681,6 +2721,7 @@ Theorem bignum_alt_thm:
    abs_ml_inv conf (Number i::stack) refs
      (Pointer a (Word (0w:α word))::roots,heap2,be,a+len+1,sp-len-1,sp1,gens) limit ts
 Proof
+  cheat (*
   rw[abs_ml_inv_def]
   \\ qmatch_assum_abbrev_tac`br = DataElement _ _ _`
   \\ `el_length br = len + 1` by
@@ -2787,7 +2828,7 @@ Proof
        \\ map_every qexists_tac [`n`,`l`] \\ rw []
        \\ ho_match_mp_tac MEM_v_all_vs
        \\ drule MEM_ZIP2 \\ rw []
-       \\ rw [EL_MEM])
+       \\ rw [EL_MEM]) *)
 QED
 
 (* update ref *)
@@ -3101,6 +3142,7 @@ Theorem update_ref_thm:
       abs_ml_inv conf (xs ++ (RefPtr b ptr)::stack) (insert ptr (ValueArray xs) refs)
         (roots,heap2,be,a,sp,sp1,gens) limit ts
 Proof
+  cheat (*
   simp_tac std_ss [abs_ml_inv_def]
   \\ rpt strip_tac \\ full_simp_tac std_ss [bc_stack_ref_inv_def]
   \\ imp_res_tac EVERY2_APPEND_CONS
@@ -3217,7 +3259,7 @@ Proof
         \\ ho_match_mp_tac MEM_v_all_vs
         \\ drule MEM_ZIP2 \\ rw []
         \\ rw [EL_MEM]))
-  \\ (full_simp_tac (srw_ss()) [INJ_DEF] \\ metis_tac [])
+  \\ (full_simp_tac (srw_ss()) [INJ_DEF] \\ metis_tac []) *)
 QED
 
 Definition heap_deref_def:
@@ -3240,6 +3282,7 @@ Theorem update_ref_thm1:
         (insert ptr (ValueArray (LUPDATE (HD xs) i xs1)) refs)
         (roots,heap2,be,a,sp,sp1,gens) limit ts
 Proof
+  cheat (*
   simp_tac std_ss [abs_ml_inv_def]
   \\ rpt strip_tac \\ full_simp_tac std_ss [bc_stack_ref_inv_def]
   \\ imp_res_tac EVERY2_APPEND_CONS
@@ -3374,7 +3417,7 @@ Proof
         \\ ho_match_mp_tac MEM_v_all_vs
         \\ drule MEM_ZIP2 \\ rw []
         \\ rw [EL_MEM]))
-  \\ full_simp_tac (srw_ss()) [INJ_DEF] \\ metis_tac []
+  \\ full_simp_tac (srw_ss()) [INJ_DEF] \\ metis_tac [] *)
 QED
 
 (* update byte ref *)
@@ -3476,6 +3519,7 @@ Theorem update_byte_ref_thm:
       abs_ml_inv conf ((RefPtr b ptr)::stack) (insert ptr (ByteArray fl ys) refs)
         (roots,h1 ++ [Bytes be fl ys ws] ++ h2,be,a,sp,sp1,gens) limit ts
 Proof
+  cheat (*
   simp_tac std_ss [abs_ml_inv_def]
   \\ rpt strip_tac \\ full_simp_tac std_ss [bc_stack_ref_inv_def]
   \\ Cases_on `roots` \\ fs [v_inv_def] \\ rpt var_eq_tac \\ fs []
@@ -3594,7 +3638,7 @@ Proof
   THEN1 (fs [INJ_DEF,FLOOKUP_DEF] \\ metis_tac [])
   \\ fs [heap_lookup_APPEND,Bytes_def,heap_length_def,el_length_def,SUM_APPEND]
   \\ rfs [] \\ rw [] \\ fs [] \\ rfs [heap_lookup_def]
-  \\ metis_tac[]
+  \\ metis_tac[] *)
 QED
 
 val heap_store_unused_thm = prove(
@@ -3671,6 +3715,7 @@ Theorem new_ref_thm:
                  (rs ++ Pointer (a+sp+sp1-(LENGTH xs + 1)) (Word 0w)::roots2,heap2,be,a,
                   sp - (LENGTH xs + 1),sp1,gens) limit ts
 Proof
+  cheat (*
   simp_tac std_ss [abs_ml_inv_def]
   \\ rpt strip_tac \\ full_simp_tac std_ss [bc_stack_ref_inv_def]
   \\ imp_res_tac EVERY2_APPEND_IMP_APPEND
@@ -3832,7 +3877,7 @@ Proof
   \\ map_every qexists_tac [`n`,`l`]
   \\ fs [lookup_insert]
   \\ ho_match_mp_tac MEM_v_all_vs
-  \\ rw []
+  \\ rw [] *)
 QED
 
 (* deref *)
@@ -3858,6 +3903,7 @@ Theorem deref_thm:
                 abs_ml_inv conf (EL n vs::RefPtr b ptr::stack) refs
                   (y::roots,heap,be,a,sp,sp1,gens) limit ts
 Proof
+  cheat (*
   full_simp_tac std_ss [abs_ml_inv_def,bc_stack_ref_inv_def]
   \\ rpt strip_tac \\ Cases_on `roots` \\ full_simp_tac (srw_ss()) [LIST_REL_def]
   \\ full_simp_tac std_ss [v_inv_def]
@@ -3909,7 +3955,7 @@ Proof
   \\ full_simp_tac (srw_ss()) [ref_edge_def,FLOOKUP_DEF,get_refs_def]
   \\ full_simp_tac (srw_ss()) [MEM_FLAT,MEM_MAP,PULL_EXISTS]
   \\ qexists_tac `(EL n l)` \\ full_simp_tac std_ss []
-  \\ full_simp_tac std_ss [MEM_EL] \\ metis_tac []
+  \\ full_simp_tac std_ss [MEM_EL] \\ metis_tac [] *)
 QED
 
 (* el *)
@@ -3984,6 +4030,7 @@ Theorem new_byte_alt_thm:
                  (Pointer a (Word 0w)::roots,heap2,be,a + ws + 1,
                   sp - (ws + 1),sp1,gens) limit ts
 Proof
+  cheat (*
   simp_tac std_ss [abs_ml_inv_def]
   \\ rpt strip_tac \\ full_simp_tac std_ss [bc_stack_ref_inv_def]
   \\ imp_res_tac EVERY2_APPEND_IMP_APPEND
@@ -4106,61 +4153,7 @@ Proof
   \\ full_simp_tac std_ss [] \\ simp_tac (srw_ss()) []
   \\ rpt strip_tac
   \\ match_mp_tac v_inv_SUBMAP \\ fs []
-  \\ fs [heap_store_rel_def,isSomeDataElement_def,PULL_EXISTS]
-QED
-
-(* pop *)
-
-Theorem pop_thm:
-   abs_ml_inv conf (xs ++ stack) refs (rs ++ roots,heap,be,a,sp,sp1,gens) limit ts /\
-    (LENGTH xs = LENGTH rs) ==>
-    abs_ml_inv conf (stack) refs (roots,heap,be,a,sp,sp1,gens) limit ts
-Proof
-  full_simp_tac std_ss [abs_ml_inv_def,bc_stack_ref_inv_def] \\ rpt strip_tac
-  \\ full_simp_tac std_ss [roots_ok_def,MEM_APPEND]
-  THEN1 (rw [] \\ res_tac \\ fs [])
-  \\ qexists_tac `f` \\ full_simp_tac std_ss []
-  \\ qexists_tac `DRESTRICT tf (all_ts refs stack)` \\ full_simp_tac std_ss []
-  \\ conj_tac
-  >- fs [INJ_DEF,DRESTRICT_DEF]
-  \\ conj_tac
-  >- fs [SUBSET_DEF,DRESTRICT_DEF]
-  \\ conj_tac
-  >- fs [SUBSET_DEF,DRESTRICT_DEF,IN_INTER]
-  \\ conj_tac
-  >- (match_mp_tac EVERY2_MEM_MONO
-     \\ imp_res_tac LIST_REL_APPEND_IMP
-     \\ first_assum(part_match_exists_tac(last o strip_conj) o concl)
-     \\ simp[FORALL_PROD] \\ rw[]
-     \\ ho_match_mp_tac v_inv_tf_restrict
-     \\ rw []
-     \\ ho_match_mp_tac MEM_in_all_ts
-     \\ qexists_tac `p_1` \\ rw []
-     \\ ho_match_mp_tac MEM_stack_all_vs
-     \\ drule MEM_ZIP2 \\ rw []
-     \\ rw [EL_MEM])
-  \\ fs[reachable_refs_def,PULL_EXISTS]
-  \\ rw[]
-  \\ fs[bc_ref_inv_def]
-  \\ fsrw_tac[boolSimps.DNF_ss][]
-  \\ first_x_assum rpt_drule
-  \\ BasicProvers.TOP_CASE_TAC \\ fs[]
-  \\ BasicProvers.TOP_CASE_TAC \\ fs[]
-  \\ BasicProvers.TOP_CASE_TAC \\ fs[] \\ rw[]
-  \\ fs[RefBlock_def,Bytes_def]
-  \\ match_mp_tac EVERY2_MEM_MONO
-  \\ imp_res_tac LIST_REL_APPEND_IMP
-  \\ first_assum(part_match_exists_tac(last o strip_conj) o concl)
-  \\ simp[FORALL_PROD] \\ rw[]
-  \\ ho_match_mp_tac v_inv_tf_restrict
-  \\ rw []
-  \\ ho_match_mp_tac MEM_in_all_ts
-  \\ qexists_tac `p_2` \\ rw []
-  \\ rw [all_vs_def] \\ disj1_tac
-  \\ map_every qexists_tac [`n`,`l`] \\ rw []
-  \\ ho_match_mp_tac MEM_v_all_vs
-  \\ drule MEM_ZIP2 \\ rw []
-  \\ rw [EL_MEM]
+  \\ fs [heap_store_rel_def,isSomeDataElement_def,PULL_EXISTS] *)
 QED
 
 (* equality *)
@@ -4224,7 +4217,8 @@ QED
 (* permute stack *)
 
 Theorem all_ts_permute:
-  ∀(refs : v ref num_map) stack stack'. PERM stack stack' ⇒ all_ts refs stack = all_ts refs stack'
+  ∀(refs : v ref num_map) stack stack'.
+    PERM stack stack' ⇒ all_ts refs stack = all_ts refs stack'
 Proof
   strip_tac
   \\ ho_match_mp_tac PERM_IND
@@ -4300,20 +4294,43 @@ Proof
   \\ fs[bc_ref_inv_def]
   \\ Cases_on `FLOOKUP f n` \\ fs []
   \\ Cases_on `lookup n refs` \\ fs []
-  \\ Cases_on `x'` \\ rw []
-  \\ qexists_tac `zs` \\ rw []
-  \\ match_mp_tac EVERY2_MEM_MONO
-  \\ imp_res_tac LIST_REL_APPEND_IMP
-  \\ first_assum(part_match_exists_tac(last o strip_conj) o concl)
-  \\ simp[FORALL_PROD] \\ rw[]
-  \\ ho_match_mp_tac v_inv_tf_restrict
-  \\ rw [] \\ ho_match_mp_tac MEM_in_all_ts
-  \\ qexists_tac `p_2` \\ rw []
-  \\ rw [all_vs_def] \\ disj1_tac
-  \\ map_every qexists_tac [`n`,`l`] \\ rw []
-  \\ ho_match_mp_tac MEM_v_all_vs
-  \\ drule MEM_ZIP2 \\ rw []
-  \\ rw [EL_MEM]
+  \\ rename [‘lookup n refs = SOME x_ref’]
+  \\ Cases_on ‘x_ref’ \\ rw []
+  >~ [‘RefBlock’] >-
+   (qexists_tac `zs` \\ rw []
+    \\ match_mp_tac EVERY2_MEM_MONO
+    \\ imp_res_tac LIST_REL_APPEND_IMP
+    \\ first_assum(part_match_exists_tac(last o strip_conj) o concl)
+    \\ simp[FORALL_PROD] \\ rw[]
+    \\ ho_match_mp_tac v_inv_tf_restrict
+    \\ rw [] \\ ho_match_mp_tac MEM_in_all_ts
+    \\ qexists_tac `p_2` \\ rw []
+    \\ rw [all_vs_def] \\ rpt disj1_tac
+    \\ map_every qexists_tac [`n`,`l`] \\ rw []
+    \\ ho_match_mp_tac MEM_v_all_vs
+    \\ drule MEM_ZIP2 \\ rw []
+    \\ rw [EL_MEM])
+  >~ [‘ThunkBlock’] >-
+   (qexists_tac `z` \\ rw []
+    \\ ho_match_mp_tac v_inv_tf_restrict
+    \\ rw [] \\ ho_match_mp_tac MEM_in_all_ts
+    \\ pop_assum $ irule_at $ Pos last
+    \\ rw [all_vs_def] \\ disj1_tac \\ disj2_tac
+    \\ first_x_assum $ irule_at $ Pos hd
+    \\ irule MEM_v_all_vs \\ simp [])
+QED
+
+(* pop *)
+
+Theorem pop_thm:
+   abs_ml_inv conf (xs ++ stack) refs (rs ++ roots,heap,be,a,sp,sp1,gens) limit ts /\
+    (LENGTH xs = LENGTH rs) ==>
+    abs_ml_inv conf (stack) refs (roots,heap,be,a,sp,sp1,gens) limit ts
+Proof
+  strip_tac
+  \\ irule (abs_ml_inv_stack_permute |> Q.SPECL [‘xs’,‘[]’] |> SRULE [])
+  \\ qexists_tac ‘ZIP(xs,rs)’
+  \\ simp [MAP_ZIP]
 QED
 
 (* duplicate *)
@@ -4366,7 +4383,9 @@ Theorem split1_thm:
     ?rs1 roots1. (roots = rs1 ++ roots1) /\ (LENGTH rs1 = LENGTH xs1)
 Proof
   full_simp_tac std_ss [abs_ml_inv_def,bc_stack_ref_inv_def,GSYM APPEND_ASSOC]
-  \\ rpt strip_tac \\ NTAC 5 (imp_res_tac LIST_REL_SPLIT1 \\ imp_res_tac LIST_REL_LENGTH) \\ metis_tac []
+  \\ rpt strip_tac
+  \\ NTAC 5 (imp_res_tac LIST_REL_SPLIT1 \\ imp_res_tac LIST_REL_LENGTH)
+  \\ metis_tac []
 QED
 
 Theorem split2_thm:
@@ -4375,7 +4394,9 @@ Theorem split2_thm:
       (LENGTH rs1 = LENGTH xs1) /\ (LENGTH rs2 = LENGTH xs2)
 Proof
   full_simp_tac std_ss [abs_ml_inv_def,bc_stack_ref_inv_def,GSYM APPEND_ASSOC]
-  \\ rpt strip_tac \\ NTAC 5 (imp_res_tac LIST_REL_SPLIT1 \\ imp_res_tac LIST_REL_LENGTH) \\ metis_tac []
+  \\ rpt strip_tac
+  \\ NTAC 5 (imp_res_tac LIST_REL_SPLIT1 \\ imp_res_tac LIST_REL_LENGTH)
+  \\ metis_tac []
 QED
 
 Theorem split3_thm:
@@ -4385,7 +4406,9 @@ Theorem split3_thm:
       (LENGTH rs3 = LENGTH xs3)
 Proof
   full_simp_tac std_ss [abs_ml_inv_def,bc_stack_ref_inv_def,GSYM APPEND_ASSOC]
-  \\ rpt strip_tac \\ NTAC 5 (imp_res_tac LIST_REL_SPLIT1 \\ imp_res_tac LIST_REL_LENGTH) \\ metis_tac []
+  \\ rpt strip_tac
+  \\ NTAC 5 (imp_res_tac LIST_REL_SPLIT1 \\ imp_res_tac LIST_REL_LENGTH)
+  \\ metis_tac []
 QED
 
 Theorem abs_ml_inv_Num:
@@ -4469,6 +4492,11 @@ Proof
   EVAL_TAC
 QED
 
+Definition thunk_tag_to_bits_def:
+  thunk_tag_to_bits Evaluated = 1w ∧
+  thunk_tag_to_bits NotEvaluated = 0w
+End
+
 Definition word_payload_def:
   (word_payload ys l (BlockTag n) qs conf =
      (* header: ...00[11] here i in ...i[11] must be 0 for the GC *)
@@ -4482,6 +4510,11 @@ Definition word_payload_def:
      (make_header conf 2w (LENGTH ys),
       MAP (word_addr conf) ys,
       (qs = []) /\ (LENGTH ys = l))) /\
+  (word_payload ys l (ThunkTag e) qs conf =
+     (* header: ...e110[11] here i in ...i[11] must be 0 for the GC *)
+     (make_header conf (thunk_tag_to_bits e << 3 || 6w) (LENGTH ys),
+      MAP (word_addr conf) ys,
+      (qs = []) /\ (LENGTH ys = 1) ∧ l = 1)) /\
   (word_payload ys l Word64Tag qs conf =
      (* header: ...011[11] here i in ...i[11] must be 1 for the GC *)
      (make_header conf 3w l,
@@ -4953,6 +4986,7 @@ Theorem all_ts_head_eq:
    v  ∈ all_vs refs stack
    ⇒ all_ts refs stack = all_ts refs (v::stack)
 Proof
+  cheat (*
   rw [FUN_EQ_THM]
   \\ EQ_TAC
   >- (rw [all_ts_def,all_vs_def] \\ metis_tac [])
@@ -4984,7 +5018,7 @@ Proof
     \\ ho_match_mp_tac v_all_vs_ts_MEM
     \\ qexists_tac `Block n0 n l`
     \\ rw [v_all_ts_def])
-  >- metis_tac []
+  >- metis_tac [] *)
 QED
 
 Theorem memory_rel_El':
@@ -5240,6 +5274,7 @@ val gc_kind_update_Ref = prove(
         (ha ++ DataElement (ys1 ++ y::ys2) l (RefTag,[])::hb) ==>
     gc_kind_inv c a sp sp1 gens
         (ha ++ DataElement (ys1 ++ z::ys2) l (RefTag,[])::hb)``,
+  cheat (*
   fs [gc_kind_inv_def] \\ every_case_tac \\ fs []
   \\ ntac 2 strip_tac THEN1
    (Cases_on `gens` \\ fs [gen_state_ok_def,EVERY_MEM]
@@ -5261,7 +5296,7 @@ val gc_kind_update_Ref = prove(
   \\ CASE_TAC \\ rw [] \\ fs [isRef_def]
   \\ fs [heap_split_def,el_length_def] \\ rfs []
   \\ rpt (CASE_TAC \\ fs [])
-  \\ rveq \\ fs [isRef_def]);
+  \\ rveq \\ fs [isRef_def] *));
 
 Theorem v_all_vs_append:
   ∀x y. v_all_vs (x ++ y) = v_all_vs x ++ v_all_vs y
@@ -7240,6 +7275,39 @@ Proof
   \\ fs [fcpTheory.FCP_BETA,word_lsl_def,word_index]
 QED
 
+Theorem memory_rel_Thunk_IMP:
+   memory_rel c be ts refs sp st m dm ((RefPtr bl p,v:'a word_loc)::vars) /\
+    lookup p refs = SOME (Thunk ev x) /\ good_dimindex (:'a) ==>
+    ?w a x.
+      v = Word w /\ w ' 0 /\ word_bit 3 x /\ ~word_bit 2 x /\ word_bit 4 x /\
+      get_real_simple_addr c st w = SOME a /\
+      get_real_addr c st w = SOME a /\
+      m a = Word x /\ a IN dm /\
+      decode_length c x = 1w /\
+      (word_bit 5 x ⇔ ev = Evaluated)
+Proof
+  fs [memory_rel_def,word_ml_inv_def,PULL_EXISTS,abs_ml_inv_def,
+      bc_stack_ref_inv_def,v_inv_def,word_addr_def] \\ rw [get_addr_0]
+  \\ `bc_ref_inv c p refs (f,tf,heap,be)` by
+    (first_x_assum match_mp_tac \\ fs [reachable_refs_def]
+     \\ qexists_tac `RefPtr bl p` \\ fs [get_refs_def])
+  \\ pop_assum mp_tac \\ simp [bc_ref_inv_def]
+  \\ fs [FLOOKUP_DEF] \\ rw []
+  \\ fs [word_addr_def,heap_in_memory_store_def]
+  \\ rpt_drule get_real_addr_get_addr \\ disch_then kall_tac
+  \\ imp_res_tac heap_lookup_SPLIT \\ clean_tac
+  \\ fs [word_heap_APPEND,word_heap_def,ThunkBlock_def,word_el_def,
+         word_payload_def,word_list_def]
+  \\ full_simp_tac (std_ss++sep_cond_ss) [cond_STAR]
+  \\ imp_res_tac EVERY2_LENGTH \\ SEP_R_TAC \\ fs [get_addr_0]
+  \\ fs [make_header_def,word_bit_def,word_or_def,fcpTheory.FCP_BETA]
+  \\ fs [good_dimindex_def]
+  \\ fs [fcpTheory.FCP_BETA,word_lsl_def,word_index]
+  \\ Cases_on ‘ev’
+  \\ fs [thunk_tag_to_bits_def]
+  \\ EVAL_TAC
+QED
+
 val expand_num =
   DECIDE ``4 = SUC 3 /\ 3 = SUC 2 /\ 2 = SUC 1 /\ 1 = SUC 0 /\
            5 = SUC 4 /\ 6 = SUC 5 /\ 7 = SUC 6 /\ 8 = SUC 7``
@@ -7866,7 +7934,7 @@ Theorem memory_rel_RefPtr_IMP':
   memory_rel c be ts refs sp st m dm ((RefPtr bl p,v)::vars) ∧
   good_dimindex (:α) ⇒
   ∃w a x.
-    v = Word w ∧ w ' 0 ∧ (word_bit 4 x ⇒ word_bit 2 x) ∧
+    v = Word w ∧ w ' 0 ∧ (* (word_bit 4 x ⇒ word_bit 2 x) ∧ *)
     (word_bit 3 x ⇔ ¬word_bit 2 x) ∧
     data_to_word_memoryProof$get_real_addr c st w = SOME a ∧
     get_real_simple_addr c st w = SOME a ∧
@@ -7874,15 +7942,16 @@ Theorem memory_rel_RefPtr_IMP':
 Proof
   strip_tac \\ drule memory_rel_RefPtr_IMP_lemma \\ strip_tac
   \\ Cases_on `res` \\ fs []
-  THEN1 (rpt_drule memory_rel_ValueArray_IMP \\ rw [] \\ fs [])
-  THEN1 (rpt_drule memory_rel_ByteArray_IMP \\ rw [] \\ fs [])
+  THEN1 (drule_all memory_rel_ValueArray_IMP \\ rw [] \\ fs [])
+  THEN1 (drule_all memory_rel_ByteArray_IMP \\ rw [] \\ fs [])
+  THEN1 (drule_all memory_rel_Thunk_IMP \\ rw [] \\ fs [])
 QED
 
 Theorem memory_rel_RefPtr_IMP:
    memory_rel c be ts refs sp st m dm ((RefPtr bl p,v:'a word_loc)::vars) /\
     good_dimindex (:'a) ==>
     ?w a x.
-      v = Word w /\ w ' 0 /\ (word_bit 4 x ==> word_bit 2 x) /\
+      v = Word w /\ w ' 0 /\ (* (word_bit 4 x ==> word_bit 2 x) /\ *)
       (word_bit 3 x <=> ~word_bit 2 x) /\
       get_real_addr c st w = SOME a /\ m a = Word x /\ a IN dm
 Proof
@@ -9838,6 +9907,7 @@ Theorem word_eq_thm0:
                 (b <=> (res = 1w)) /\
                 l <= l1 + (LENGTH v1 + SUM (MAP vb_size v1)) * dimword (:'a))
 Proof
+  cheat (*
   ho_match_mp_tac do_eq_ind \\ rpt conj_tac
   \\ once_rewrite_tac [do_eq_def] \\ simp []
   THEN1 (* do_eq Numbers *)
@@ -10129,7 +10199,7 @@ Proof
                (CONJUNCT2 word_eq_min_max_clock)
   \\ PURE_ONCE_REWRITE_TAC[MAX_COMM]
   \\ fs[ETA_THM]
-  \\ fs[LEFT_ADD_DISTRIB]
+  \\ fs[LEFT_ADD_DISTRIB] *)
 QED
 
 Theorem word_eq_thm:
@@ -12005,6 +12075,7 @@ Theorem cons_multi_thm:
                   ++ heap2, be,
             a + heap_length Allocd, sp - heap_length Allocd, sp1, gens) limit (ts + LENGTH xs)
 Proof
+  cheat (*
   rw [abs_ml_inv_def]
   \\ qpat_x_assum `bc_stack_ref_inv _ _ _ _ _` mp_tac
   \\ simp [Once bc_stack_ref_inv_def] \\ strip_tac
@@ -12309,7 +12380,7 @@ Proof
   \\ qpat_x_assum `LENGTH xs = _` (assume_tac o GSYM)
   \\ rw []
   \\ match_mp_tac (Q.INST [`sp`|->`sp+sp1`] (SPEC_ALL v_inv_list_to_v))
-  \\ unlength_tac [heap_expand_def]
+  \\ unlength_tac [heap_expand_def] *)
 QED
 
 Theorem memory_rel_append:
@@ -13823,14 +13894,14 @@ Proof
          >-
           (simp [AllCaseEqs()]
            \\ rw [] \\ gvs [SF SFY_ss]
-           \\ gvs [Bytes_def,isRef_def])
+           \\ gvs [Bytes_def,isRef_def,isMutTag_def])
          \\ gvs [heap_split_def,el_length_Bytes]
          \\ IF_CASES_TAC \\ gvs []
-         >- (rw [] \\ gvs [isRef_def,Bytes_def])
+         >- (rw [] \\ gvs [isRef_def,Bytes_def,isMutTag_def])
          \\ IF_CASES_TAC \\ gvs []
          \\ simp [AllCaseEqs()]
          \\ rpt strip_tac \\ gvs []
-         \\ gvs [Bytes_def,isRef_def])
+         \\ gvs [Bytes_def,isRef_def,isMutTag_def])
       \\ ‘unused_space_inv a (sp' + sp1) heap1’ by
         (gvs [unused_space_inv_def,SF DNF_ss]
          \\ gvs [data_up_to_def]
@@ -13844,7 +13915,7 @@ Proof
          \\ IF_CASES_TAC \\ simp []
          \\ simp [AllCaseEqs()]
          \\ rw [] \\ gvs [SF SFY_ss]
-         \\ gvs [Bytes_def,isRef_def])
+         \\ gvs [Bytes_def,isRef_def,isMutTag_def])
       \\ ‘all_ts (insert p2 (ByteArray fl2 res_vals) refs) =
           all_ts refs’ by
         (gvs [all_ts_def,FUN_EQ_THM,lookup_insert,CaseEq"bool"]
